regex/Regex/Syntax/Parser/ToString.lean
@@ -97,7 +97,13 @@ def Ast.toString : Ast → String
   | .group ast => s!"({ast.toString})"
   | .alternate ast1 ast2 => s!"{ast1.toString}|{ast2.toString}"
   | .concat ast1 ast2 => s!"{ast1.toString}{ast2.toString}"
-  | .star ast => s!"{ast.toString}*"
+  | .repeat 0 .none ast => s!"{ast.toString}*"
+  | .repeat 1 .none ast => s!"{ast.toString}+"
+  | .repeat 0 (.some 1) ast => s!"{ast.toString}?"
+  | .repeat min (.some max) ast => 
+    if min == max then ast.toString ++ "{" ++ Nat.repr min ++ "}"
+    else ast.toString ++ "{" ++ Nat.repr min ++ "," ++ Nat.repr max ++ "}"
+  | .repeat min .none ast => ast.toString ++ "{" ++ Nat.repr min ++ ",}"
   | .classes cs => Classes.toString cs
   | .perl pc => s!"\\{PerlClass.toString pc}"
   | .dot => "."
